<p class=MsoBodyText style='margin-bottom:20.0pt;text-justify:
inter-ideograph;line-height:12.7pt'><span class=BodyTextChar>Now it is clear
that Theorem 1 follows from the Lemma 2 below:</span></p>

<p class=MsoBodyText style='margin-bottom:0in;text-justify:
inter-ideograph;line-height:12.7pt'><span class=BodyTextChar>LEMMA 2. </span><span
class=BodyTextChar><i>There exists an algorithm which for any given Turing
machine T and its input λ</i> </span><span class=BodyTextChar><i>constructs a
finite presentation of group H with the following properties:</i></span></p>

<p class=MsoBodyText style='margin-bottom:0in;text-justify:
inter-ideograph;text-indent:0in;line-height:12.5pt'><span class=BodyTextChar>(1)
</span><span class=BodyTextChar><i>There exists an element h </i></span><span
class=BodyTextChar><span style='font-family:"Cambria Math",serif'>∈ </span></span><span
class=BodyTextChar><i>H such that H/[h, H] = {e};</i></span></p>

<p class=MsoBodyText style='margin-bottom:0in;text-justify:
inter-ideograph;text-indent:0in;line-height:12.75pt'><span class=BodyTextChar>(2)
</span><span class=BodyTextChar><i>The second homology group of H is trivial;</i></span></p>

<p class=MsoBodyText style='margin-bottom:14.0pt;text-justify:
inter-ideograph;text-indent:0in;line-height:12.75pt'><span class=BodyTextChar>(3)</span><span
class=BodyTextChar><i> H is trivial if and only if T eventually halts when it
starts its work with λ.</i></span></p>

<p class=MsoBodyText style='margin-bottom:20.0pt;text-justify:
inter-ideograph;line-height:12.75pt'><span class=BodyTextChar><i>Proof.</i> In
many proofs of the algorithmic unsolvability of the word problem for finitely
presented groups one actually describes an algorithm constructing for a given
Turing machine </span><span class=BodyTextChar><i>T</i> and its input </span><span
class=BodyTextChar><i>λ</i> a finite presentation of a group </span><span
class=BodyTextChar><i>G</i> and a word representing an element </span><span
class=BodyTextChar><i>w </i></span><span class=BodyTextChar><span
style='font-family:"Segoe UI Symbol",sans-serif'>∈ </span></span><span
class=BodyTextChar><i>G</i> such that </span><span class=BodyTextChar><i>w</i>
= </span><span class=BodyTextChar><i>e</i> in </span><span class=BodyTextChar><i>G</i>
if and only if </span><span class=BodyTextChar><i>T</i> eventually halts, when
it starts its work with the input </span><span class=BodyTextChar><i>λ</i> (cf.
[R], [AC]). The Adian-Rabin “witness” construction (cf. [M], pp. 13-14) enables
one to construct a finite presentation of a group </span><span
class=BodyTextChar><i>G<sub>w</sub></i> such that </span><span
class=BodyTextChar><i>G<sub>w</sub></i> is trivial if and only if </span><span
class=BodyTextChar><i>w</i> = </span><span class=BodyTextChar><i>e</i> in </span><span
class=BodyTextChar><i>G</i>. Moreover, if </span><span class=BodyTextChar><i>w
≠ e</i> in </span><span class=BodyTextChar><i>G</i> then </span><span
class=BodyTextChar><i>G</i> embeds in </span><span class=BodyTextChar><i>G<sub>w</sub>.</i>
To get this finite presentation one adds to the list of generators of </span><span
class=BodyTextChar><i>G</i> (denoted by </span><span class=BodyTextChar><i>x</i><sub>1</sub>,…,
</span><span class=BodyTextChar><i>x<sub>k</sub></i>) 3 new generators </span><span
class=BodyTextChar><i>a, b, c </i>and to the list of relations of </span><span
class=BodyTextChar><i>G</i> the following (</span><span class=BodyTextChar><i>k</i>
+ 3) new relations:</span></p>

<p class=MsoBodyText style='margin-bottom:14.0pt;text-justify:
inter-ideograph;line-height:normal'><span class=BodyTextChar><i>a</i><sup>-1</sup></span><span
class=BodyTextChar><i>ba = c</i><sup>-1</sup></span><span class=BodyTextChar><i>b</i><sup>-1</sup></span><span
class=BodyTextChar><i>cbc&nbsp;&nbsp;&nbsp;
</i>(1)</span></p>

<p class=MsoBodyText style='margin-bottom:14.0pt;text-justify:
inter-ideograph;line-height:normal'><span class=BodyTextChar><i>a</i><sup>-2</sup></span><span
class=BodyTextChar><i>b</i><sup>-1</sup></span><span class=BodyTextChar><i>aba</i><sup>2</sup></span><span
class=BodyTextChar><i> = c<sup>-</sup></i><sup>2</sup></span><span
class=BodyTextChar><i>b<sup>-</sup></i><sup>1</sup></span><span
class=BodyTextChar><i>cbc</i><sup>2</sup></span><span class=BodyTextChar><i><sup>&nbsp;&nbsp;&nbsp;
</sup></i>(2) </span></p>

<p class=MsoBodyText style='margin-bottom:14.0pt;text-justify:
inter-ideograph;line-height:normal'><span class=BodyTextChar><i>a<sup>-</sup></i><sup>3</sup>[</span><span
class=BodyTextChar><i>w, b</i>]</span><span class=BodyTextChar><i>a</i><sup>3</sup></span><span
class=BodyTextChar><i> = c<sup>-</sup></i><sup>3</sup></span><span
class=BodyTextChar><i>bc</i><sup>3</sup></span><span class=BodyTextChar><i><sup>&nbsp;&nbsp;&nbsp;&nbsp;&nbsp;&nbsp;&nbsp;&nbsp;&nbsp;&nbsp;&nbsp;&nbsp;&nbsp;&nbsp;&nbsp;&nbsp;&nbsp;
</sup></i>(3)</span></p>

<p class=MsoBodyText style='margin-bottom:20.0pt;text-justify:
inter-ideograph;line-height:normal'><span class=BodyTextChar><i>a<sup>-</sup></i><sup>(3</sup></span><span
class=BodyTextChar><i><sup>+i</sup></i><sup>)</sup></span><span
class=BodyTextChar><i> x<sub>i</sub>ba</i><sup>(3</sup></span><span
class=BodyTextChar><i><sup>+i</sup></i><sup>)</sup></span><span
class=BodyTextChar><i><sup> </sup>=c<sup>-</sup></i><sup>(</sup></span><span
class=BodyTextChar><i><sup>3+i</sup></i><sup>)</sup></span><span
class=BodyTextChar><i>bc</i><sup>(</sup></span><span class=BodyTextChar><i><sup>3+i</sup></i><sup>)</sup></span><span
class=BodyTextChar><i> &nbsp;&nbsp;i </i>= 1,2,…,</span><span
class=BodyTextChar><i> k.&nbsp;&nbsp;&nbsp;&nbsp;&nbsp;&nbsp;&nbsp; </i>(4)</span></p>

<p class=MsoBodyText style='margin-bottom:3.0pt;text-justify:
inter-ideograph;line-height:12.8pt'><span class=BodyTextChar>It is not
difficult to see (and the proof is given in [M] on pp. 14-15) that the normal
closure of </span><span class=BodyTextChar><i>w</i> in </span><span
class=BodyTextChar><i>G<sub>w</sub></i> is </span><span class=BodyTextChar><i>G<sub>w</sub>.</i>
(This fact is used in [M] to demonstrate that </span><span class=BodyTextChar><i>G<sub>w
</sub></i>is trivial if </span><span class=BodyTextChar><i>w</i> = </span><span
class=BodyTextChar><i>e</i> in </span><span class=BodyTextChar><i>G</i>.) The
proof uses only the relations (1)-(4) and goes as follows: Obviously, [</span><span
class=BodyTextChar><i>w,b</i>] belongs to the normal closure of </span><span
class=BodyTextChar><i>w.</i> Hence, (3) implies that </span><span
class=BodyTextChar><i>b</i> belongs to the normal closure of </span><span
class=BodyTextChar><i>w.</i> Now (4) implies that for any </span><span
class=BodyTextChar><i>i, x<sub>i</sub></i> belongs to the normal closure of </span><span
class=BodyTextChar><i>w,</i> and (1) implies that </span><span
class=BodyTextChar><i>c</i> belongs to the normal closure of </span><span
class=BodyTextChar><i>w.</i> Now (2) implies that </span><span
class=BodyTextChar><i>a</i> belongs to the normal closure of </span><span
class=BodyTextChar><i>w</i>.</span></p>

<p class=MsoBodyText style='margin-bottom:14.0pt;text-justify:
inter-ideograph;line-height:12.8pt'><span class=BodyTextChar>The relations
(1)-(4) can be rewritten in the following equivalent form:</span></p>

<p class=Tableofcontents0 style='margin-bottom:8.0pt;
text-justify:inter-ideograph'><span class=Tableofcontents>[<i>bca</i><sup>-1</sup><i>,
b</i>]<i> = cb</i><sup>-1</sup>&nbsp;&nbsp;&nbsp;&nbsp;&nbsp;&nbsp;&nbsp;&nbsp;&nbsp;&nbsp; (1')</span></p>

<p class=Tableofcontents0 style='margin-bottom:8.0pt;
text-justify:inter-ideograph'><span class=Tableofcontents>[<i>bc</i><sup>2</sup><i>a</i><sup>-2</sup><i>b</i><sup>-1</sup><i>,
a</i>]<i> = ca</i><sup>-1</sup>&nbsp;&nbsp;&nbsp;&nbsp; (2')</span></p>

<p class=Tableofcontents0 style='margin-bottom:8.0pt;
text-justify:inter-ideograph'><span class=Tableofcontents>[<i>c</i><sup>3</sup><i>a</i>
<sup>-3</sup><i>, </i>[<i>w, b</i>]][<i>w, b</i>]<i>=b</i>&nbsp;&nbsp;&nbsp;&nbsp;&nbsp;&nbsp;&nbsp;&nbsp;&nbsp;&nbsp;&nbsp;&nbsp;&nbsp;&nbsp;&nbsp;&nbsp;&nbsp;&nbsp;&nbsp;&nbsp;&nbsp; (3')</span></p>

<p class=Tableofcontents0 style='margin-bottom:14.0pt;
text-justify:inter-ideograph'><span class=Tableofcontents><i>x<sub>i </sub>= </i>[<i>a</i><sup>(3<i>
+ i</i>)</sup><i>c<sup>-</sup></i><sup>(3<i> + i</i>)</sup><i>,b</i>]<i>,&nbsp;&nbsp;&nbsp;&nbsp;&nbsp;&nbsp;&nbsp;&nbsp;&nbsp;&nbsp;&nbsp; i
= </i>1,2,…,<i>k</i>.&nbsp;&nbsp;&nbsp;&nbsp;&nbsp; (4')</span></p>

<p class=Tableofcontents0 style='margin-bottom:14.0pt;
text-justify:inter-ideograph'><span class=Tableofcontents>Using (3') one can
replace (1') by the following equivalent relation:</span></p>

<p class=Tableofcontents0 style='margin-bottom:14.0pt;
text-justify:inter-ideograph'><span class=Tableofcontents><i>c</i>[<i>b,</i> <i>w</i>][[<i>w</i>,<i>b</i>],
<i>c</i><sup>3</sup><i>a<sup>-</sup></i><sup>3</sup>][<i>b, bca</i><sup>-1</sup>]=<i>
e,</i>&nbsp;&nbsp;&nbsp;&nbsp;&nbsp;&nbsp;&nbsp;&nbsp;&nbsp;&nbsp;&nbsp;&nbsp;&nbsp;&nbsp;&nbsp;&nbsp;&nbsp;&nbsp; (1&quot;)</span></p>

<p class=Tableofcontents0 style='margin-bottom:14.0pt;
text-justify:inter-ideograph;text-indent:0in'><span class=Tableofcontents>and
then replace (2') by the following equivalent relation:</span></p>

<p class=Tableofcontents0 style='margin-bottom:14.0pt;
text-justify:inter-ideograph;text-indent:16.0pt'><span class=Tableofcontents><i>a</i>[<i>b,</i>
<i>w</i>][[<i>w</i>, <i>b</i>], <i>c</i><sup>3</sup><i>a</i><sup>-3</sup>][<i>b</i>,<i>
bca</i><sup>-1</sup>][<i>bc</i><sup>2</sup><i>a</i><sup>-2</sup><i>b</i><sup>-1</sup><i>,
a</i>]<i> = e.</i>&nbsp;&nbsp;&nbsp;&nbsp;&nbsp;&nbsp;&nbsp;&nbsp;&nbsp;&nbsp;&nbsp;&nbsp;&nbsp;&nbsp;&nbsp;&nbsp;&nbsp;&nbsp; (2&quot;)</span></p>
